[llir-semantics] Progress on closures

StoreToLoad.v
@@ -3,6 +3,7 @@
 (* (C) 2020 Nandor Licker. All rights reserved. *)
 
 Require Import Coq.ZArith.ZArith.
+Require Import Coq.NArith.NArith.
 Require Import Coq.Lists.List.
 
 Require Import LLIR.Aliasing.
@@ -16,39 +17,141 @@ Require Import LLIR.Dom.
 
 Import ListNotations.
 
+Definition propagate_loads (f: func) (rs: reaching_stores) (aa: points_to_set): list (reg * reg) :=
+  PTrie.values (reg * reg) (PTrie.map_opt inst (reg * reg) 
+    (fun k inst =>
+      match inst with
+      | LLLd addr dst next =>
+        match get_load_addr aa addr with
+        | Some obj => 
+          match get_store_to rs k obj with
+          | Some src => Some (dst, src)
+          | None => None
+          end
+        | None => None
+        end
+      | _ => None
+      end
+    ) f.(fn_insts)).
 
-Section PROPAGATION.
+Fixpoint closure_chain (src: reg) (pairs: list (reg * reg)): (option reg * list (reg * reg)) :=
+  match pairs with
+  | nil => (None, nil)
+  | (dst', src') :: pairs' =>
+    match dst' =? src with
+    | true => (Some src', pairs')
+    | false => 
+      match closure_chain src pairs' with
+      | (None, pairs'') => (None, nil)
+      | (v, pairs'') => (v, (dst', src') :: pairs'')
+      end
+    end
+  end.
+
+Theorem closure_chain_length:
+  forall (pairs: list (reg * reg)) (src: reg) (p: reg * reg),
+    Nat.lt (length (snd (closure_chain src (p::pairs)))) (S (length pairs)).
+Proof.
+  induction pairs; try intros.
+  { 
+    unfold closure_chain.
+    destruct p.
+    destruct (r =? src); simpl; apply Nat.lt_0_1.
+  }
+  {
+    simpl.
+    destruct p.
+    destruct (r =? src); try apply Nat.lt_succ_diag_r.
+    destruct a.
+    destruct (r1 =? src) eqn:E; try apply Nat.lt_succ_diag_r.
+    destruct (closure_chain src pairs) eqn:Hc.
+    destruct o.
+    + simpl.
+      rewrite <- Nat.succ_lt_mono.
+      generalize (IHpairs src (r1, r1)).
+      unfold closure_chain.
+      rewrite E.
+      fold closure_chain.
+      intro H.
+      rewrite Hc in H.
+      simpl in H.
+      apply H.
+    + simpl.
+      apply Nat.lt_0_succ.
+  }
+Qed.
+
+Program Fixpoint closure_step (src: reg) (pairs: list (reg * reg)) { measure (length pairs) } :=
+  match closure_chain src pairs with
+  | (None, _) => src
+  | (Some v, pairs') => closure_step v pairs'
+  end.
+Obligation 1.
+  rename Heq_anonymous into Heq.
+  unfold closure_chain in Heq.
+  destruct pairs.
+  - inversion Heq.
+  - destruct p as [x y].
+    destruct (x =? src) eqn:Ex.
+    {
+      inversion Heq.
+      simpl.
+      apply Nat.lt_succ_r.
+      reflexivity.
+    }
+    {
+      fold closure_chain in Heq.
+      simpl.
+      destruct (closure_chain src pairs) eqn:E.
+      destruct o.
+      - inversion Heq.
+        assert ((x, y) :: l = snd (closure_chain src ((x, y) :: pairs))).
+        {
+          simpl.
+          rewrite Ex.
+          rewrite E.
+          simpl.
+          reflexivity.
+        }
+        rewrite H.
+        apply closure_chain_length.
+      - inversion Heq.
+    }
+Qed.
+
+Definition closure (pairs: list (reg * reg)): list (reg * reg) :=
+  List.map 
+    (fun pair =>
+      match pair with
+      | (dst, src) => (dst, closure_step src pairs)
+      end)
+    pairs.
+
+Definition propagate_store_to_load (f: func): func :=
+  let aa := local_pta f in
+  let rs := analyse_reaching_stores f aa in
+  let loads := closure (propagate_loads f rs aa) in
+  mkfunc f.(fn_args) f.(fn_stack) f.(fn_insts) f.(fn_phis) f.(fn_entry).
+
+Section PROPERTIES.
   Variable f: func.
   Variable rs: reaching_stores.
   Variable aa: points_to_set.
 
-  Definition get_propagated_loads: list (reg * reg) :=
-    PTrie.values (reg * reg) (PTrie.map_opt inst (reg * reg) 
-      (fun k inst =>
-        match inst with
-        | LLLd addr dst next =>
-          match get_load_addr aa addr with
-          | Some obj => 
-            match get_store_to rs k obj with
-            | Some src => Some (dst, src)
-            | None => None
-            end
-          | None => None
-          end
-        | _ => None
-        end
-      ) f.(fn_insts)).
+  Hypothesis H_f_valid: is_valid f.
 
   Lemma propagate_src_dst:
-    forall (dst: reg) (src: reg),
-      In (dst, src) get_propagated_loads ->
+    forall (loads: list (reg * reg)) (dst: reg) (src: reg),
+      loads = propagate_loads f rs aa ->
+      In (dst, src) loads ->
         exists (k: node) (addr: reg) (object: positive) (offset: positive),
           loads_from f aa k dst addr object offset /\
           store_to_at rs k src object offset.
   Proof.
-    intros src dst.
-    intros Helem.
-    unfold get_propagated_loads in Helem.
+    intros loads src dst.
+    intro Hprop.
+    intro Helem.
+    rewrite Hprop in Helem.
     apply PTrie.values_correct in Helem.
     destruct Helem as [k Helem].
     exists k.
@@ -70,33 +173,36 @@ Section PROPAGATION.
     - apply store. symmetry. apply Hstore.
   Qed.
 
+  Definition reg_dom (src: reg) (dst: reg): Prop :=
+    forall (def: node) (use: node),
+      DefinedAt f def src ->
+      UsedAt f use dst ->
+      Dominates f def use.
+
   Lemma src_dominates_dst:
-    is_valid f ->
-      forall (src: reg) (dst: reg),
-        In (dst, src) get_propagated_loads -> 
-          forall (def: node) (use: node),
-            DefinedAt f def src ->
-            UsedAt f use dst ->
-            Dominates f def use.
+    forall (loads: list (reg * reg)) (src: reg) (dst: reg),
+      loads = propagate_loads f rs aa ->
+      In (dst, src) loads -> reg_dom src dst.
   Proof.
-    intros Hvalid.
-    intros src dst.
-    intros Helem.
-    apply propagate_src_dst in Helem.
+    intros loads src dst.
+    intro Hprop.
+    intro Helem.
+    apply (propagate_src_dst loads dst src Hprop) in Helem.
     destruct Helem as [k Helem].
     destruct Helem as [ld_addr Helem].
     destruct Helem as [object Helem].
     destruct Helem as [offset Helem].
     destruct Helem as [Hload Hstore].
-    assert (Hstore': store_to_at rs k src object offset). { apply Hstore. }
+    assert (Hstore': store_to_at rs k src object offset).
+    { apply Hstore. }
     apply (reaching_store_origin f aa) in Hstore'.
     destruct Hstore' as [store Hstore'].
     destruct Hstore' as [val Hstore'].
     destruct Hstore' as [next Hstore'].
     destruct Hstore' as [Hstore' Hdom].
     inversion Hstore'.
-    assert (Hvalid': is_valid f). { apply Hvalid. }
-    destruct Hvalid' as [Hdef_dom_uses Hdefs_unique].
+    assert (H_f_valid': is_valid f). { apply H_f_valid. }
+    destruct H_f_valid' as [Hdef_dom_uses Hdefs_unique].
     intros def use.
     intros Hdef_src.
     intros Huse_dst.
@@ -147,7 +253,7 @@ Section PROPAGATION.
             (def_inst := LLLd ld_addr dst next1)
             (use_inst := i)
             (r := dst).
-          - apply Hvalid.
+          - apply H_f_valid.
           - apply H6.
           - unfold Defs. reflexivity.
           - symmetry. apply Euse.
@@ -160,11 +266,51 @@ Section PROPAGATION.
       }
     }
   Qed.
-End PROPAGATION.
 
-Definition propagate_store_to_load (f: func): func :=
-  let aa := local_pta f in
-  let rs := analyse_reaching_stores f aa in
-  let loads := get_propagated_loads f rs aa in
-  mkfunc f.(fn_args) f.(fn_stack) f.(fn_insts) f.(fn_phis) f.(fn_entry).
+  Lemma propagate_load_unique:
+    forall (loads: list (reg * reg)) (dst: reg) (src: reg),
+      loads = propagate_loads f rs aa ->
+      In (dst, src) loads ->
+        forall (src': reg), In (dst, src') loads -> src = src'.
+  Proof.
+    intros loads  dst src.
+    intro Hloads.
+    intro Hin.
+    intro src'.
+    intro Hin'.
+    generalize (propagate_src_dst loads dst src Hloads Hin).
+    intros Hexists.
+    generalize (propagate_src_dst loads dst src' Hloads Hin').
+    intros Hexists'.
+    destruct Hexists as [k [addr [object [offset [Hload Hstore]]]]].
+    destruct Hexists' as [k' [addr' [object' [offset' [Hload' Hstore']]]]].
+    inversion Hload.
+    assert (Hdef: Defs (LLLd addr dst next) dst). reflexivity.
+    destruct H_f_valid as [_ Hunique].
+    inversion Hload'.
+    generalize (Hunique k' (LLLd addr' dst next0) dst H7 Hdef (LLLd addr dst next) k).
+    intro Huniq.
+    assert (Heq: k = k' /\ LLLd addr dst next = LLLd addr' dst next0).
+    {
+      apply Huniq.
+      split.
+      - apply H0.
+      - simpl. reflexivity.
+    }
+    destruct Heq as [Hk_eq Hld_eq].
+    inversion Hld_eq as [Haddr].
+    rewrite <- Haddr in H6.
+    rewrite <- H6 in H.
+    inversion H.
+    rewrite <- H15 in Hstore'.
+    rewrite <- H16 in Hstore'.
+    inversion Hstore.
+    inversion Hstore'.
+    rewrite <- Hk_eq in H21.
+    rewrite <- H14 in H21.
+    inversion H21.
+    reflexivity.
+  Qed.
+End PROPERTIES.
+
 
